Updates.

LC/NV/UTLC/Sub/ReplaceFree.lean
@@ -1,4 +1,4 @@
-import LC.NV.UTLC.Term
+import LC.NV.UTLC.Binders
 
 
 set_option autoImplicit false
@@ -7,23 +7,23 @@ set_option autoImplicit false
 open Term_
 
 
--- replace_free u e1 e2 := e2 [ u := e1 ]
--- u -> e1 in e2
+-- replace_free u N M := M [ u := N ]
+-- u -> N in M
 def replace_free
 (u : Symbol_)
-(e : Term_) :
+(N : Term_) :
 Term_ → Term_
 | var_ x =>
   if u = x
-  then e
+  then N
   else var_ x
 
-| app_ P Q => app_ (replace_free u e P) (replace_free u e Q)
+| app_ P Q => app_ (replace_free u N P) (replace_free u N Q)
 
 | abs_ x P =>
   if u = x
   then abs_ x P
-  else abs_ x (replace_free u e P)
+  else abs_ x (replace_free u N P)
 
 
 -------------------------------------------------------------------------------
@@ -31,10 +31,10 @@ Term_ → Term_
 
 lemma replace_free_self
   (u : Symbol_)
-  (e : Term_) :
-  replace_free u (var_ u) e = e :=
+  (M : Term_) :
+  replace_free u (var_ u) M = M :=
   by
-    induction e
+    induction M
     case var_ x =>
       unfold replace_free
       split_ifs
@@ -54,6 +54,101 @@ lemma replace_free_self
       case neg c1 =>
         rw [ih]
 
+
+lemma not_free_in_replace_free_self
+  (u : Symbol_)
+  (N : Term_)
+  (M : Term_)
+  (h1 : ¬ is_free_in u M) :
+  replace_free u N M = M :=
+  by
+    induction M
+    case var_ x =>
+      unfold is_free_in at h1
+      unfold replace_free
+      split_ifs
+      rfl
+    case app_ P Q ih_1 ih_2 =>
+      unfold is_free_in at h1
+      simp at h1
+      obtain ⟨h1_left, h1_right⟩ := h1
+
+      unfold replace_free
+      rw [ih_1 h1_left]
+      rw [ih_2 h1_right]
+    case abs_ x P ih =>
+      unfold is_free_in at h1
+      simp at h1
+
+      unfold replace_free
+      split_ifs
+      case pos c1 =>
+        rfl
+      case neg c1 =>
+        specialize h1 c1
+        specialize ih h1
+        rw [ih]
+
+
+lemma replace_free_inverse
+  (u v : Symbol_)
+  (M : Term_)
+  (h1 : ¬ occurs_in v M) :
+  replace_free v (var_ u) (replace_free u (var_ v) M) = M :=
+  by
+    induction M
+    case var_ x =>
+      unfold occurs_in at h1
+
+      simp only [replace_free]
+      split_ifs
+      case pos c1 =>
+        rw [c1]
+        unfold replace_free
+        simp
+      case neg c1 =>
+        unfold replace_free
+        split_ifs
+        rfl
+    case app_ P Q ih_1 ih_2 =>
+      unfold occurs_in at h1
+      simp at h1
+      obtain ⟨h1_left, h1_right⟩ := h1
+
+      simp only [replace_free]
+      rw [ih_1 h1_left]
+      rw [ih_2 h1_right]
+    case abs_ x P ih =>
+      unfold occurs_in at h1
+      simp at h1
+      obtain ⟨h1_left, h1_right⟩ := h1
+      specialize ih h1_right
+
+      simp only [replace_free]
+      split_ifs
+      case pos c1 =>
+        unfold replace_free
+        split_ifs
+        have s1 : ¬ is_free_in v P :=
+        by
+          intro contra
+          apply h1_right
+          exact is_free_in_imp_occurs_in v P contra
+        obtain s2 := not_free_in_replace_free_self v (var_ u) P s1
+        rw [s2]
+      case neg c1 =>
+        unfold replace_free
+        split_ifs
+        rw [ih]
+
+
+lemma not_is_free_in_replace_free
+  (u v : Symbol_)
+  (M : Term_)
+  (h1 : ¬ u = v) :
+  ¬ is_free_in u (replace_free u (var_ v) M) :=
+  by
+    sorry
 
 /-
 theorem fastReplaceFree_self
